ExistentialRules/ChaseSequence/ChaseDerivation.lean
@@ -321,29 +321,10 @@ theorem constants_node_subset_constants_fs_union_constants_rules
         apply Or.inl
         rw [List.mem_flatMap] at c_mem
         rcases c_mem with ⟨t, t_mem, c_mem⟩
-        rw [List.mem_map] at t_mem
-        rcases t_mem with ⟨v, v_mem, t_mem⟩
-        rcases FunctionFreeConjunction.mem_vars.mp (origin.fst.val.rule.frontier_subset_vars_body v_mem) with ⟨a, a_mem, v_mem'⟩
-        exists origin.fst.val.subs.apply_function_free_atom a
-        constructor
-        . apply (cd2.active_trigger_origin_next next_mem).left
-          rw [List.mem_toSet]
-          apply TermMapping.apply_generalized_atom_mem_apply_generalized_atom_list
-          exact a_mem
-        . unfold Fact.constants
-          rw [List.mem_flatMap]
-          exists t
-          constructor
-          . unfold GroundSubstitution.apply_function_free_atom
-            unfold TermMapping.apply_generalized_atom
-            rw [List.mem_map]
-            exists VarOrConst.var v
-            constructor
-            . exact v_mem'
-            . unfold PreTrigger.subs_for_mapped_head at t_mem
-              rw [PreTrigger.apply_to_var_or_const_frontier_var _ _ _ _ v_mem] at t_mem
-              exact t_mem
-          . exact c_mem
+        apply FactSet.constants_subset_of_subset (cd2.active_trigger_origin_next next_mem).left
+        rw [FactSet.mem_constants_iff_mem_terms]; exists t; constructor
+        . rw [FactSet.mem_terms_toSet]; apply PreTrigger.mem_terms_mapped_body_of_mem_mapped_frontier; exact t_mem
+        . exact c_mem
       | inr c_mem =>
         apply Or.inr
         exists origin.fst.val.rule
